move things around a little; prove first new typed-writing

theories/typing/programs.v
@@ -43,6 +43,16 @@ Section typing.
     (∀ tid qE, □ (lft_ctx -∗ elctx_interp E qE -∗ llctx_interp L 1 -∗ tctx_interp tid T1 -∗
                    WP e {{ v, elctx_interp E qE ∗ llctx_interp L 1 ∗ tctx_interp tid (T2 v) }}))%I.
   Global Arguments typed_instruction _ _ _ _%E _.
+
+  (** Writing and Reading **)
+  Definition typed_writing (E : elctx) (L : llctx) (ty1 ty ty2 : type) : Prop :=
+    ∀ p tid Φ E, lftE ∪ (↑lrustN) ⊆ E →
+      lft_ctx -∗ tctx_elt_interp tid (TCtx_hasty p ty1) -∗
+      (∀ (l:loc) vl,
+         ⌜length vl = ty.(ty_size)⌝ -∗ ⌜eval_path p = Some #l⌝ -∗ l ↦∗ vl -∗
+           (∀ vl', l ↦∗ vl' -∗ ▷ (ty.(ty_own) tid vl') ={E}=∗
+                           tctx_elt_interp tid (TCtx_hasty p ty2)) -∗ Φ #l) -∗
+      WP p @ E {{ Φ }}.
 End typing.
 
 Notation typed_instruction_ty E L T1 e ty := (typed_instruction E L T1 e (λ v : val, [TCtx_hasty v ty])).
