theories/typing/bool.v
@@ -11,6 +11,10 @@ Section bool.
 
   Global Instance bool_send : Send bool.
   Proof. iIntros (tid1 tid2 vl). done. Qed.
+End bool.
+
+Section typing.
+  Context `{typeG Σ}.
 
   Lemma type_bool (b : Datatypes.bool) E L :
     typed_instruction_ty E L [] #b bool.
@@ -26,10 +30,10 @@ Section bool.
     (* FIXME why can't I merge these two iIntros? *)
     iIntros (He1 He2). iIntros (tid qE) "#LFT HE HL HC".
     rewrite tctx_interp_cons. iIntros "[Hp HT]".
-    wp_bind p. iApply (wp_hasty with "Hp"). iIntros (v) "[% Hown]".
+    wp_bind p. iApply (wp_hasty with "Hp"). iIntros (v) "% Hown".
     iDestruct "Hown" as (b) "Hv". iDestruct "Hv" as %[=->].
     destruct b; wp_if.
     - iApply (He1 with "LFT HE HL HC HT").
     - iApply (He2 with "LFT HE HL HC HT").
   Qed.
-End bool.
+End typing.
